translator/lean/corellzk2smt/Corellzk2smt/FFConstraints/Basic_th.lean
@@ -1,4 +1,5 @@
 import Corellzk2smt.FFConstraints.Basic
+import Corellzk2smt.Config
 
 /- This module defines the syntax of constraint systems over finite fields
    and boolean variables -/
@@ -7,8 +8,9 @@ namespace Corellzk2smt.FFConstraints.Basic_th
 open Corellzk2smt.FFConstraints.Basic
 
 /- fetchMacro returns a smaller list of macros -/
-theorem fetchMacroLT {c : ZKConfig} (ms ms' : List (FFMacro c)) (name : String) (m : FFMacro c) :
-  fetchMacro ms name = Except.ok (m, ms') → ms'.length < ms.length := by
+theorem fetchMacroLT {c : ZKConfig} (gconf : GlobalConfig c) (ms ms' : List (FFMacro c))
+    (name : String) (m : FFMacro c) :
+  fetchMacro gconf ms name = Except.ok (m, ms') → ms'.length < ms.length := by
   cases ms with
   | nil => simp [fetchMacro]
   | cons head tail =>
@@ -21,7 +23,7 @@ theorem fetchMacroLT {c : ZKConfig} (ms ms' : List (FFMacro c)) (name : String) 
       · simp only [h, not_false_eq_true, beq_iff_eq, ↓reduceIte, List.length_cons,
         Order.lt_add_one_iff] at *
         intro h1
-        have h2 := fetchMacroLT tail ms' name m h1
+        have h2 := fetchMacroLT gconf tail ms' name m h1
         grind
 
 end Corellzk2smt.FFConstraints.Basic_th
